Iris/Iris/Instances/Lib/CInvariants.lean
@@ -20,65 +20,69 @@ public import Iris.Std.List
 
 namespace Iris
 
-open BI CMRA OFE Iris Std LawfulSet Excl Fraction COFE
+open BI CMRA OFE Iris Std LawfulSet Excl COFE
 
 /-! # Cancelable Invariants -/
 
-abbrev CInvF (F : Type _) : OFunctorPre :=
-  ProdOF (constOF (Option (Excl Unit))) (constOF (Option (Frac F)))
+abbrev CInvF : OFunctorPre :=
+  ProdOF (constOF (Option (Excl Unit))) (constOF (Option Qp))
 
 @[rocq_alias cinvG]
-class CInvG (F : Type _) [UFraction F] (GF : BundledGFunctors) where
-  inv : ElemG GF (CInvF F)
+class CInvG (GF : BundledGFunctors) where
+  inv : ElemG GF CInvF
 
 attribute [reducible, instance] CInvG.inv
 
 namespace CancelableInvariant
 
-variable {F : Type _} [UFraction F]
-variable {GF : BundledGFunctors} [InvGS_gen hlc GF] [W : CInvG F GF]
+variable {GF : BundledGFunctors} [InvGS_gen hlc GF] [W : CInvG GF]
+
+private theorem qpOne_valid : ✓ (One.one : Qp) := by
+  show (One.one : Qp).val ≤ 1
+  have : (One.one : Qp).val = 1 := rfl
+  grind
 
 @[rocq_alias cinv_own]
-def own (γ : GName) (p : Frac F) : IProp GF := iOwn (E := W.inv) γ (none, some p)
+def own (γ : GName) (p : Qp) : IProp GF := iOwn (E := W.inv) γ (none, some p)
 
 @[rocq_alias cinv_excl]
 def excl (γ : GName) : IProp GF := iOwn (E := W.inv) γ (some (Excl.excl ()), none)
 
 @[rocq_alias cinv]
 def cinv (N : Namespace) (γ : GName) (P : IProp GF) : IProp GF :=
-  inv N iprop(P ∗ excl (F := F) γ ∨ own γ (⟨One.one⟩ : Frac F))
+  inv N iprop(P ∗ excl γ ∨ own γ (One.one : Qp))
 
 /-! ## Instances -/
 
 @[rocq_alias cinv_own_timeless]
-instance instTimelessOwn (γ : GName) (p : Frac F) : Timeless (own (GF := GF) γ p) :=
+instance instTimelessOwn (γ : GName) (p : Qp) : Timeless (own (GF := GF) γ p) :=
   iOwn_timeless
 
-instance instTimelessExcl (γ : GName) : Timeless (excl (F := F) (GF := GF) γ) :=
+instance instTimelessExcl (γ : GName) : Timeless (excl (GF := GF) γ) :=
   iOwn_timeless
 
 @[rocq_alias cinv_contractive]
 instance instContractiveCinv (N : Namespace) (γ : GName) :
-    Contractive (cinv (GF := GF) (F := F) N γ) where
+    Contractive (cinv (GF := GF) N γ) where
   distLater_dist {n x y} H := by
     unfold cinv
     refine Contractive.distLater_dist fun m hm => or_ne.ne (sep_ne.ne (H _ hm) .rfl) .rfl
 
 @[rocq_alias cinv_ne]
 instance instNonExpansiveCinv (N : Namespace) (γ : GName) :
-    NonExpansive (cinv (F := F) (GF := GF) N γ) :=
+    NonExpansive (cinv (GF := GF) N γ) :=
   ne_of_contractive _
 
 #rocq_ignore cinv_proper "Subsumed by instNonExpansiveCinv"
 
 @[rocq_alias cinv_persistent]
 instance instPersistentCinv (N : Namespace) (γ : GName) (P : IProp GF) :
-    Persistent (cinv (F := F) N γ P) := by
+    Persistent (cinv N γ P) := by
   unfold cinv; infer_instance
 
 @[rocq_alias cinv_own_valid]
-theorem own_valid {γ : GName} {q1 q2 : Frac F} :
-    ⊢@{IProp GF} own γ q1 -∗ own γ q2 -∗ ⌜Proper (q1.car + q2.car)⌝ := by
+theorem own_valid {γ : GName} {q1 q2 : Qp} :
+    ⊢@{IProp GF} own γ q1 -∗ own γ q2 -∗ ⌜(q1 + q2).val ≤ 1⌝ := by
   unfold own
   iintro H1 H2
   ihave H := iOwn_op $$ [H1 H2]; iframe
@@ -89,25 +93,25 @@ theorem own_valid {γ : GName} {q1 q2 : Frac F} :
 
 @[rocq_alias cinv_own_fractional]
 instance instFractionalOwn (γ : GName) :
-    Fractional (fun p : F => own (GF := GF) γ ⟨p⟩) where
+    Fractional (fun p : Qp => own (GF := GF) γ p) where
   fractional p q := by
-    show iOwn (E := W.inv) γ ((none, some ⟨p + q⟩)) ⊣⊢ _
+    show iOwn (E := W.inv) γ ((none, some (p + q))) ⊣⊢ _
     refine .trans ?_ iOwn_op
     exact equiv_iff.mp (NonExpansive.eqv (.of_eq rfl))
 
 @[rocq_alias cinv_own_as_fractional]
-instance instAsFractionalOwn (γ : GName) (q : F) :
-    AsFractional (own (GF := GF) γ ⟨q⟩) (fun p : F => own γ ⟨p⟩) q where
+instance instAsFractionalOwn (γ : GName) (q : Qp) :
+    AsFractional (own (GF := GF) γ q) (fun p : Qp => own γ p) q where
   as_fractional := .rfl
   as_fractional_fractional := instFractionalOwn γ
 
 @[rocq_alias cinv_own_excl_alloc]
 theorem own_excl_alloc (P : GName → Prop) (HP : PredInfinite P) :
-    ⊢@{IProp GF} |==> ∃ γ, ⌜P γ⌝ ∗ excl (F := F) γ ∗ own γ (⟨One.one⟩ : Frac F) := by
+    ⊢@{IProp GF} |==> ∃ γ, ⌜P γ⌝ ∗ excl γ ∗ own γ (One.one : Qp) := by
   imod iOwn_alloc_strong (E := W.inv)
-    ((some (Excl.excl ()), none) • (none, some (⟨One.one⟩ : Frac F)) :
-      CInvF F (IProp GF) (IProp GF)) P ?_
-    ⟨trivial, UFraction.one_whole.1⟩ with ⟨%γ, %HPγ, Hown⟩
+    ((some (Excl.excl ()), none) • (none, some (One.one : Qp)) :
+      CInvF (IProp GF) (IProp GF)) P ?_
+    ⟨trivial, qpOne_valid⟩ with ⟨%γ, %HPγ, Hown⟩
   · intro N
     obtain ⟨γ, HPγ, Hγ⟩ := HP (List.range (N + 1))
     exact ⟨γ, by grind, HPγ⟩
@@ -120,15 +124,15 @@ theorem own_excl_alloc (P : GName → Prop) (HP : PredInfinite P) :
     iframe
 
 @[rocq_alias cinv_own_1_l]
-theorem own_one_l {γ : GName} {q : Frac F} :
-    ⊢ own (GF := GF) γ (⟨One.one⟩ : Frac F) -∗ own γ q -∗ False := by
+theorem own_one_l {γ : GName} {q : Qp} :
+    ⊢ own (GF := GF) γ (One.one : Qp) -∗ own γ q -∗ False := by
   iintro H1 H2
   icases own_valid $$ H1 H2 with %H
-  exact (UFraction.one_whole.2 ⟨q.car, H⟩).elim
+  exact absurd H (by have := q.2; have : (One.one : Qp).val = 1 := rfl; grind)
 
 @[rocq_alias cinv_excl_excl]
 theorem excl_excl (γ : GName) :
-    ⊢ excl (GF := GF) (F := F) γ -∗ excl (F := F) γ -∗ False := by
+    ⊢ excl (GF := GF) γ -∗ excl γ -∗ False := by
   iintro H1 H2
   ihave H := iOwn_op $$ [H1 H2]
   · unfold excl; iframe
@@ -138,7 +142,7 @@ theorem excl_excl (γ : GName) :
 
 @[rocq_alias cinv_iff]
 nonrec theorem cinv_iff {N : Namespace} {γ : GName} {P Q : IProp GF} :
-    ⊢ cinv (GF := GF) (F := F) N γ P -∗ ▷ □ (P ↔ Q) -∗ cinv (F := F) N γ Q := by
+    ⊢ cinv (GF := GF) N γ P -∗ ▷ □ (P ↔ Q) -∗ cinv N γ Q := by
   unfold cinv
   iintro HI #⟨HPQ₁, HPQ₂⟩
   iapply inv_iff $$ HI
@@ -157,9 +161,9 @@ nonrec theorem cinv_iff {N : Namespace} {γ : GName} {P Q : IProp GF} :
 
 @[rocq_alias cinv_alloc_strong]
 theorem alloc_strong (P : GName → Prop) (HP : PredInfinite P) (E : CoPset) (N : Namespace) :
-    ⊢@{IProp GF} |={E}=> ∃ γ, ⌜P γ⌝ ∗ own γ (⟨One.one⟩ : Frac F) ∗
-      ∀ Q, ▷ Q ={E}=∗ cinv (F := F) N γ Q := by
-  imod own_excl_alloc (F := F) P HP with ⟨%γ, %HPγ, Hexcl, Hown⟩
+    ⊢@{IProp GF} |={E}=> ∃ γ, ⌜P γ⌝ ∗ own γ (One.one : Qp) ∗
+      ∀ Q, ▷ Q ={E}=∗ cinv N γ Q := by
+  imod own_excl_alloc P HP with ⟨%γ, %HPγ, Hexcl, Hown⟩
   imodintro
   iexists γ
   iframe %HPγ Hown
@@ -173,15 +177,15 @@ theorem alloc_strong (P : GName → Prop) (HP : PredInfinite P) (E : CoPset) (N 
 @[rocq_alias cinv_alloc_strong_open]
 theorem alloc_strong_open (P : GName → Prop) (HP : PredInfinite P) (E : CoPset) (N : Namespace)
   (Hsub : ↑N ⊆ E) :
-    ⊢@{IProp GF} |={E}=> ∃ γ, ⌜P γ⌝ ∗ own (F := F) γ (⟨One.one⟩ : Frac F) ∗
-      ∀ (Q : IProp GF), |={E, E \ ↑N}=> cinv (F := F) N γ Q ∗ (▷ Q ={E \ ↑N, E}=∗ True) := by
-  imod own_excl_alloc (F := F) P HP with ⟨%γ, %HPγ, Hexcl, Hown⟩
+    ⊢@{IProp GF} |={E}=> ∃ γ, ⌜P γ⌝ ∗ own γ (One.one : Qp) ∗
+      ∀ (Q : IProp GF), |={E, E \ ↑N}=> cinv N γ Q ∗ (▷ Q ={E \ ↑N, E}=∗ True) := by
+  imod own_excl_alloc P HP with ⟨%γ, %HPγ, Hexcl, Hown⟩
   imodintro
   iexists γ
   iframe %HPγ Hown
   iframe
   iintro %Q
-  imod inv_alloc_open N E iprop(Q ∗ excl (F := F) γ ∨ own γ (⟨One.one⟩ : Frac F)) Hsub with ⟨HI, Hclose⟩
+  imod inv_alloc_open N E iprop(Q ∗ excl γ ∨ own γ (One.one : Qp)) Hsub with ⟨HI, Hclose⟩
   imodintro
   unfold cinv
   iframe
@@ -193,15 +197,15 @@ theorem alloc_strong_open (P : GName → Prop) (HP : PredInfinite P) (E : CoPset
 
 @[rocq_alias cinv_alloc_cofinite]
 theorem alloc_cofinite (G : List GName) (E : CoPset) (N : Namespace) :
-    ⊢@{IProp GF} |={E}=> ∃ γ, ⌜γ ∉ G⌝ ∗ own (F := F) γ (⟨One.one⟩ : Frac F) ∗
-      ∀ Q, ▷ Q ={E}=∗ cinv (F := F) N γ Q :=
+    ⊢@{IProp GF} |={E}=> ∃ γ, ⌜γ ∉ G⌝ ∗ own γ (One.one : Qp) ∗
+      ∀ Q, ▷ Q ={E}=∗ cinv N γ Q :=
   alloc_strong (· ∉ G) (PredInfinite.not_mem G) E N
 
 @[rocq_alias cinv_alloc]
 theorem alloc (E : CoPset) (N : Namespace) (P : IProp GF) :
-    ⊢ ▷ P ={E}=∗ ∃ γ, cinv (F := F) N γ P ∗ own γ (⟨One.one⟩ : Frac F) := by
+    ⊢ ▷ P ={E}=∗ ∃ γ, cinv N γ P ∗ own γ (One.one : Qp) := by
   iintro HP
-  imod alloc_cofinite (F := F) [] E N with ⟨%γ, %Hγ, Hown, Halloc⟩
+  imod alloc_cofinite [] E N with ⟨%γ, %Hγ, Hown, Halloc⟩
   imod Halloc $$ HP with HI
   imodintro
   iexists γ
@@ -209,9 +213,9 @@ theorem alloc (E : CoPset) (N : Namespace) (P : IProp GF) :
 
 @[rocq_alias cinv_alloc_open]
 theorem alloc_open (E : CoPset) (N : Namespace) (P : IProp GF) (Hsub : ↑N ⊆ E) :
-    ⊢@{IProp GF} |={E, E \ ↑N}=> ∃ γ, cinv (F := F) N γ P ∗ own γ (⟨One.one⟩ : Frac F) ∗
+    ⊢@{IProp GF} |={E, E \ ↑N}=> ∃ γ, cinv N γ P ∗ own γ (One.one : Qp) ∗
       (▷ P ={E \ ↑N, E}=∗ True) := by
-  imod alloc_strong_open (F := F) (fun _ => True) PredInfinite.true E N Hsub
+  imod alloc_strong_open (fun _ => True) PredInfinite.true E N Hsub
     with ⟨%γ, _, Hown, Hmake⟩
   imod Hmake $$ %P with ⟨HI, Hclose⟩
   imodintro
@@ -219,10 +223,10 @@ theorem alloc_open (E : CoPset) (N : Namespace) (P : IProp GF) (Hsub : ↑N ⊆ 
   iframe
 
 @[rocq_alias cinv_acc_strong]
-theorem acc_strong (E : CoPset) (N : Namespace) (γ : GName) (p : Frac F) (P : IProp GF)
+theorem acc_strong (E : CoPset) (N : Namespace) (γ : GName) (p : Qp) (P : IProp GF)
     (Hsub : ↑N ⊆ E) :
-    ⊢ cinv (F := F) N γ P -∗ own γ p ={E, E \ ↑N}=∗
-      ▷ P ∗ own γ p ∗ ∀ (E' : CoPset), ▷ P ∨ own γ (⟨One.one⟩ : Frac F) ={E', ↑N ∪ E'}=∗ True := by
+    ⊢ cinv N γ P -∗ own γ p ={E, E \ ↑N}=∗
+      ▷ P ∗ own γ p ∗ ∀ (E' : CoPset), ▷ P ∨ own γ (One.one : Qp) ={E', ↑N ∪ E'}=∗ True := by
   unfold cinv
   iintro #Hinv Hown
   imod inv_acc_strong _ _ _ Hsub $$ Hinv with ⟨(⟨HP, >Hexcl⟩ | >Hown'), Hclose⟩
@@ -237,9 +241,9 @@ theorem acc_strong (E : CoPset) (N : Namespace) (γ : GName) (p : Frac F) (P : I
     iapply own_one_l $$ Hown' Hown
 
 @[rocq_alias cinv_acc]
-theorem acc (E : CoPset) (N : Namespace) (γ : GName) (p : Frac F) (P : IProp GF)
+theorem acc (E : CoPset) (N : Namespace) (γ : GName) (p : Qp) (P : IProp GF)
     (Hsub : ↑N ⊆ E) :
-    ⊢ cinv (F := F) N γ P -∗ own γ p ={E, E \ ↑N}=∗ ▷ P ∗ own γ p ∗ (▷ P ={E \ ↑N, E}=∗ True) := by
+    ⊢ cinv N γ P -∗ own γ p ={E, E \ ↑N}=∗ ▷ P ∗ own γ p ∗ (▷ P ={E \ ↑N, E}=∗ True) := by
   iintro #Hinv Hγ
   imod acc_strong _ _ _ _ _ Hsub $$ Hinv Hγ with ⟨HP, Hγ, Hcl⟩
   imodintro
@@ -253,8 +257,8 @@ theorem acc (E : CoPset) (N : Namespace) (γ : GName) (p : Frac F) (P : IProp GF
 
 @[rocq_alias cinv_acc_1]
 theorem acc_one (E : CoPset) (N : Namespace) (γ : GName) (P : IProp GF) (Hsub : ↑N ⊆ E) :
-    ⊢ cinv (F := F) N γ P -∗ own (F := F) γ (⟨One.one⟩ : Frac F) ={E}=∗
-      ▷ P ∗ (▷ P ={E}=∗ own γ (⟨One.one⟩ : Frac F)) := by
+    ⊢ cinv N γ P -∗ own γ (One.one : Qp) ={E}=∗
+      ▷ P ∗ (▷ P ={E}=∗ own γ (One.one : Qp)) := by
   iintro #Hinv Hγ
   unfold cinv
   imod inv_acc _ _ _ Hsub $$ Hinv with ⟨(⟨HP, >Hexcl⟩ | >Hγ'), Hclose⟩
@@ -275,7 +279,7 @@ theorem acc_one (E : CoPset) (N : Namespace) (γ : GName) (P : IProp GF) (Hsub :
 
 @[rocq_alias cinv_cancel]
 theorem cancel (E : CoPset) (N : Namespace) (γ : GName) (P : IProp GF) (Hsub : ↑N ⊆ E) :
-    ⊢ cinv (F := F) N γ P -∗ own (F := F) γ (⟨One.one⟩ : Frac F) ={E}=∗ ▷ P := by
+    ⊢ cinv N γ P -∗ own γ (One.one : Qp) ={E}=∗ ▷ P := by
   iintro #Hinv Hγ
   imod acc_one _ _ _ _ Hsub $$ Hinv Hγ with ⟨HP, -⟩
   imodintro
